formalization/ContextualHOL.lean
@@ -2,3 +2,4 @@ import ContextualHOL.Syntax
 import ContextualHOL.Elab
 import ContextualHOL.Core
 import ContextualHOL.CorePrinter
+import ContextualHOL.Substitution
